src/impl/TLS13.Impl.ConnectionState.Queries.fsti
@@ -496,6 +496,8 @@ fn select_supported_server_parameters_runtime
                   CS.server_key_share_public =
                     CryptoSpec.x25519_public_from_private
                       (Ghost.reveal server_private_key);
+                  CS.server_p256_private = None;
+                  CS.server_p256_public = CS.server_p256_absent;
                   CS.server_selected_credential =
                     cfg.CS.server_credential_identity;
                 } in
