src/impl/TLS13.Impl.Server.Driver.BufferedHandshake.fst
@@ -96,6 +96,8 @@ let lemma_select_server_parameters_ready_can_select
             CS.server_key_share_public =
               CryptoSpec.x25519_public_from_private
                 (CL.raw_slice payload 32 64);
+            CS.server_p256_private = None;
+            CS.server_p256_public = CS.server_p256_absent;
             CS.server_selected_credential =
               (Some?.v st.CS.cs_model.CS.model_config.CS.config_server). CS.server_credential_identity;
           })
@@ -133,6 +135,8 @@ let lemma_select_server_parameters_input_ready_intro
              CS.server_key_share_private = Some server_private_key;
              CS.server_key_share_public =
                CryptoSpec.x25519_public_from_private server_private_key;
+             CS.server_p256_private = None;
+             CS.server_p256_public = CS.server_p256_absent;
              CS.server_selected_credential =
                cfg.CS.server_credential_identity;
            }
@@ -183,6 +187,8 @@ let lemma_select_server_parameters_call_ready
             CS.server_key_share_public =
               CryptoSpec.x25519_public_from_private
                 (CL.raw_slice payload 32 64);
+            CS.server_p256_private = None;
+            CS.server_p256_public = CS.server_p256_absent;
             CS.server_selected_credential =
               (Some?.v st.CS.cs_model.CS.model_config.CS.config_server). CS.server_credential_identity;
           })
@@ -1185,6 +1191,8 @@ let lemma_select_derive_success_server_hello_ready
         CS.server_key_share_private = Some server_private_key;
         CS.server_key_share_public =
           CryptoSpec.x25519_public_from_private server_private_key;
+        CS.server_p256_private = None;
+        CS.server_p256_public = CS.server_p256_absent;
         CS.server_selected_credential =
           cfg.CS.server_credential_identity;
       } in
@@ -1207,6 +1215,8 @@ let lemma_select_derive_success_server_hello_ready
     CS.server_key_share_private = Some server_private_key;
     CS.server_key_share_public =
       CryptoSpec.x25519_public_from_private server_private_key;
+    CS.server_p256_private = None;
+    CS.server_p256_public = CS.server_p256_absent;
     CS.server_selected_credential =
       server_cfg.CS.server_credential_identity;
   } in
