src/impl/TLS13.Impl.Server.Driver.BufferedHandshake.fsti
@@ -59,6 +59,8 @@ val lemma_select_server_parameters_input_ready_intro
              CS.server_key_share_private = Some server_private_key;
              CS.server_key_share_public =
                CryptoSpec.x25519_public_from_private server_private_key;
+             CS.server_p256_private = None;
+             CS.server_p256_public = CS.server_p256_absent;
              CS.server_selected_credential =
                cfg.CS.server_credential_identity;
            }
@@ -89,6 +91,8 @@ let selection_from_payload_correct
        CS.server_key_share_private = Some (CL.raw_slice payload 32 64);
        CS.server_key_share_public =
          CryptoSpec.x25519_public_from_private (CL.raw_slice payload 32 64);
+       CS.server_p256_private = None;
+       CS.server_p256_public = CS.server_p256_absent;
        CS.server_selected_credential =
          cfg.CS.server_credential_identity;
      } in
